src/program_proof/mvcc/txn_proof.v
@@ -63,6 +63,40 @@ Proof using EqDecision0 H H0 H1 H2 H3 H4 H5 H6 K M.
   by rewrite list_delete_insert_delete.
 Qed.
 
+Lemma list_swap_with_end {A} (l : list A) (i : nat) (xlast xi : A) :
+  (i < pred (length l))%nat ->
+  last l = Some xlast ->
+  l !! i = Some xi ->
+  <[i := xlast]> (removelast l) ≡ₚ delete i l.
+Proof.
+  intros Hlt Hlast Hi.
+  apply last_Some in Hlast as [l' El].
+  rewrite El.
+  assert (Hlen : length l' = pred (length l)).
+  { rewrite El. rewrite last_length. lia. }
+  (* RHS *)
+  rewrite delete_take_drop.
+  rewrite take_app_le; last lia.
+  rewrite drop_app_le; last lia.
+  (* LHS *)
+  rewrite removelast_last.
+  rewrite insert_take_drop; last lia.
+  apply Permutation_app_head.
+  apply Permutation_cons_append.
+Qed.
+
+Lemma list_insert_at_end {A} (l : list A) (x : A) :
+  l ≠ [] ->
+  <[pred (length l) := x]> l = (removelast l) ++ [x].
+Proof.
+  intros Hnotnil.
+  destruct (@nil_or_length_pos A l); first contradiction.
+  rewrite insert_take_drop; last lia.
+  rewrite -removelast_firstn_len.
+  replace (S _) with (length l); last lia.
+  by rewrite drop_all.
+Qed.
+
 End lemmas.
 
 Section heap.
@@ -104,6 +138,8 @@ Definition wrent := (u64 * (bool * u64) * loc)%type.
 Definition wrent_to_val (x : wrent) :=
   (#x.1.1, (#x.1.2.1, (#x.1.2.2, #()), (#x.2, #())))%V.
 
+(* TODO: [site_active_tids_half_auth γ sid (gset_to_gmap () (list_to_set tidsactiveL))] to remove [tidsactiveM] *)
+
 Definition own_txnsite (txnsite : loc) (sid : u64) γ : iProp Σ := 
   ∃ (tidlast tidmin : u64) (tidsactive : Slice.t)
     (tidsactiveL : list u64) (tidsactiveM : gmap u64 unit),
@@ -112,6 +148,7 @@ Definition own_txnsite (txnsite : loc) (sid : u64) γ : iProp Σ :=
     "HactiveL" ∷ typed_slice.is_slice tidsactive uint64T 1 tidsactiveL ∗
     "HactiveAuth" ∷ site_active_tids_half_auth γ sid tidsactiveM ∗
     "%HactiveLM" ∷ ⌜(list_to_set tidsactiveL) = dom (gset u64) tidsactiveM⌝ ∗
+    "%HactiveND" ∷ (⌜NoDup tidsactiveL⌝) ∗
     "HminAuth" ∷ site_min_tid_half_auth γ sid (int.nat tidmin) ∗
     "%HtidOrder" ∷ (⌜Forall (λ tid, int.Z tidmin ≤ int.Z tid ≤ int.Z tidlast) (tidlast :: tidsactiveL)⌝) ∗
     "%HtidFree" ∷ (∀ tid, ⌜int.Z tidlast < int.Z tid -> tid ∉ dom (gset u64) tidsactiveM⌝) ∗
@@ -299,6 +336,8 @@ Proof using mvcc_ghostG0.
       { (* TODO: Prove [HactiveAuth]. *) admit. }
       iSplitL.
       { iPureIntro. set_solver. }
+      iSplit.
+      { iPureIntro. apply NoDup_nil_2. }
       iSplit.
       { (*TODO: Prove [HminAuth]. *) admit. }
       iSplit; iPureIntro.
@@ -576,7 +615,7 @@ Proof.
   set P := λ (b : bool), (∃ (tidnew : u64),
              "Htidlast" ∷ site ↦[TxnSite :: "tidLast"] #tidlast ∗
              "HtidRef" ∷ tidRef ↦[uint64T] #tidnew ∗
-             "%Hexit" ∷ if b then ⌜True⌝ else ⌜(int.Z tidnew) > (int.Z tidlast)⌝)%I.
+             "%Hexit" ∷ if b then True else ⌜(int.Z tidnew) > (int.Z tidlast)⌝)%I.
   wp_apply (wp_forBreak_cond P with "[] [Htidlast HtidRef]").
   { clear Φ.
     iIntros (Φ) "!> Hloop HΦ".
@@ -616,6 +655,8 @@ Proof.
   iIntros (tidsactive') "HactiveL".
   wp_storeField.
   wp_loadField.
+
+  (* The local set of active tids is added with [tid], prove [tid ≥ tidmin]. *)
 
   (* Open the global invariant. *)
   iApply fupd_wp.
@@ -666,9 +707,21 @@ Proof.
       rewrite dom_insert_L.
       set_solver.
     }
-    iSplit.
+    iPureIntro.
+    split.
+    { (* Prove [HactiveND]. *)
+      apply NoDup_app.
+      split; first done.
+      split; last apply NoDup_singleton.
+      intros tidx Hin.
+      rewrite -HactiveLM in HtidFree.
+      setoid_rewrite not_elem_of_list_to_set in HtidFree.
+      assert (contra : tidnew ∉ tidsactiveL).
+      { apply HtidFree. word. }
+      set_solver.
+    }
+    split.
     { (* Prove [HtidOrder]. *)
-      iPureIntro.
       apply Forall_cons.
       split.
       { split; last done.
@@ -684,9 +737,8 @@ Proof.
       apply (Forall_impl _ _ _ HtidOrder).
       word.
     }
-    iSplit; last done.
+    split; last done.
     { (* Prove [HtidlastNotin]. *)
-      iPureIntro.
       simpl.
       intros tidx Htidx.
       subst tidsactiveM'.
@@ -711,17 +763,219 @@ Proof.
   iPureIntro. word.
 Qed.
 
-Definition spec_swapWithEnd (xs : list u64) := xs.
-
 (*****************************************************************)
 (* func swapWithEnd(xs []uint64, i uint64)                       *)
 (*****************************************************************)
-Local Theorem wp_swapWithEnd (xsS : Slice.t) (xs : list u64) (i : u64) :
-  {{{ typed_slice.is_slice xsS uint64T 1 xs }}}
-    TxnMgr__getMinActiveTIDSite (to_val xsS) #i
-  {{{ RET #(); typed_slice.is_slice xsS uint64T 1 (spec_swapWithEnd xs) }}}.
+Local Theorem wp_swapWithEnd (xsS : Slice.t) (xs : list u64) (i : u64) (x : u64) :
+  {{{ typed_slice.is_slice xsS uint64T 1 xs ∧ (⌜xs !! (int.nat i) = Some x⌝) }}}
+    swapWithEnd (to_val xsS) #i
+  {{{ (xs' : list u64), RET #(); typed_slice.is_slice xsS uint64T 1 (xs' ++ [x]) ∧
+                                 (⌜xs' ≡ₚ delete (int.nat i) xs⌝)
+  }}}.
 Proof.
-Admitted.
+  iIntros (Φ) "[HtidsS %Hlookup] HΦ".
+  wp_call.
+  iDestruct (is_slice_sz with "HtidsS") as "%HtidsSz".
+  iDestruct (typed_slice.is_slice_small_acc with "HtidsS") as "[HtidsS HtidsC]".
+  rewrite fmap_length in HtidsSz.
+  assert (Hgz : int.Z xsS.(Slice.sz) > 0).
+  { apply lookup_lt_Some in Hlookup. word. }
+
+  (***********************************************************)
+  (* tmp := xs[len(xs) - 1]                                  *)
+  (***********************************************************)
+  wp_apply wp_slice_len.
+  wp_pures.
+  set idxlast := word.sub _ _.
+  assert (Hidxlast : int.Z idxlast = (int.Z xsS.(Slice.sz)) - 1).
+  { subst idxlast. word. }
+  assert (HlookupLast : (int.nat idxlast < length xs)%nat) by word.
+  apply list_lookup_lt in HlookupLast as [xlast HlookupLast].
+  (* wp_apply (typed_slice.wp_SliceGet (V:=u64) with "[HtidsS]"). *)
+  wp_apply (typed_slice.wp_SliceGet with "[$HtidsS]").
+  { iFrame.
+    iPureIntro.
+    by rewrite HlookupLast.
+  }
+  iIntros "HtidsS".
+    
+  (***********************************************************)
+  (* xs[len(xs) - 1] = xs[i]                                 *)
+  (***********************************************************)
+  wp_pures.
+  wp_apply (typed_slice.wp_SliceGet with "[$HtidsS]").
+  { iFrame.
+    iPureIntro.
+    by rewrite Hlookup.
+  }
+  iIntros "HtidsS".
+  wp_apply wp_slice_len.
+  wp_pures.
+  wp_apply (typed_slice.wp_SliceSet with "[$HtidsS]").
+  { iFrame.
+    iPureIntro.
+    by rewrite HlookupLast.
+  }
+  iIntros "HtidsS".
+  wp_pures.
+
+  (***********************************************************)
+  (* xs[i] = tmp                                             *)
+  (***********************************************************)
+  wp_apply (typed_slice.wp_SliceSet with "[$HtidsS]").
+  { iFrame.
+    iPureIntro.
+    apply lookup_lt_is_Some_2.
+    rewrite insert_length.
+    by eapply lookup_lt_Some.
+  }
+  iIntros "HtidsS".
+  iDestruct ("HtidsC" with "HtidsS") as "HtidsS".
+  wp_pures.
+
+  destruct (decide (pred (length xs) ≤ int.nat i)%nat).
+  - (* Case: [i = idxlast]. *)
+    iApply "HΦ".
+    iModIntro.
+    subst idxlast.
+    replace (int.nat (word.sub _ _)) with (pred (length xs)) in *; last word.
+    apply lookup_lt_Some in Hlookup as Hlt.
+    { assert (Ei : (int.nat i) = pred (length xs)) by lia.
+      rewrite Ei.
+      rewrite list_insert_insert.
+      rewrite list_insert_at_end; last set_solver.
+      replace x with xlast; last first.
+      { rewrite Ei in Hlookup. set_solver. }
+      iFrame.
+      iPureIntro.
+      rewrite delete_take_drop.
+      replace (drop _ _) with ([] : list u64); last first.
+      { replace (S _) with (length xs); last lia. by rewrite drop_all. }
+      rewrite app_nil_r.
+      by rewrite removelast_firstn_len.
+    }
+  - (* Case: [i ≠ idxlast]. *)
+    iApply "HΦ".
+    iModIntro.
+    apply Nat.nle_gt in n.
+    replace (int.nat (word.sub _ _)) with (pred (length xs)); last word.
+    rewrite list_insert_at_end; last set_solver.
+    rewrite insert_app_l; last first.
+    { rewrite removelast_firstn_len. rewrite take_length_le; word. }
+    iFrame.
+    iPureIntro.
+    apply list_swap_with_end with x; [done | | done].
+    rewrite -HlookupLast.
+    replace (int.nat idxlast) with (pred (length xs)); last word.
+    apply last_lookup.
+Qed.
+
+(*****************************************************************)
+(* func findTID(tid uint64, tids []uint64) uint64                *)
+(*****************************************************************)
+Local Theorem wp_findTID (tid : u64) (tidsS : Slice.t) (tids : list u64) :
+  {{{ typed_slice.is_slice tidsS uint64T 1 tids ∗ ⌜tid ∈ tids⌝ }}}
+    findTID #tid (to_val tidsS)
+  {{{ (idx : u64), RET #idx; typed_slice.is_slice tidsS uint64T 1 tids ∧ (⌜tids !! (int.nat idx) = Some tid⌝) }}}.
+Proof.
+  iIntros (Φ) "[HtidsS %Helem] HΦ".
+  wp_call.
+
+  (***********************************************************)
+  (* var idx uint64 = 0                                      *)
+  (***********************************************************)
+  wp_apply (wp_ref_to); first auto.
+  iIntros (idxRef) "HidxRef".
+  wp_pures.
+  
+  (***********************************************************)
+  (* for {                                                   *)
+  (*     tidx := tids[idx]                                   *)
+  (*     if tid == tidx {                                    *)
+  (*         break                                           *)
+  (*     }                                                   *)
+  (*     idx++                                               *)
+  (* }                                                       *)
+  (***********************************************************)
+  set P := λ (b : bool), (∃ (idx : u64),
+    "HidxRef" ∷ idxRef ↦[uint64T] #idx ∗
+    "HtidsS" ∷  typed_slice.is_slice tidsS uint64T 1 tids ∗
+    "%Hne" ∷ (⌜Forall (λ tidx, tidx ≠ tid) (take (int.nat idx) tids)⌝) ∗
+    "%Hbound" ∷ ⌜(int.Z idx < Z.of_nat (length tids))⌝ ∗
+    "%Hexit" ∷ (⌜if b then True else tids !! (int.nat idx) = Some tid⌝))%I.
+  wp_apply (wp_forBreak P with "[] [HidxRef HtidsS]").
+  { clear Φ.
+    iIntros (Φ) "!> Hloop HΦ".
+    iNamed "Hloop".
+    wp_pures.
+    wp_load.
+    assert (Hlookup : (int.nat idx < length tids)%nat) by word.
+    apply list_lookup_lt in Hlookup as [tidx Hlookup].
+    iDestruct (is_slice_small_acc with "HtidsS") as "[HtidsS HtidsC]".
+    wp_apply (wp_SliceGet with "[HtidsS]").
+    { iFrame.
+      iPureIntro.
+      rewrite list_lookup_fmap.
+      by rewrite Hlookup.
+    }
+    iIntros "[HtidsS %HtidsVT]".
+    iDestruct ("HtidsC" with "HtidsS") as "HtidsS".
+    wp_pures.
+    wp_if_destruct.
+    { iApply "HΦ". unfold P. eauto with iFrame. }
+    wp_load.
+    wp_store.
+    iApply "HΦ".
+    iModIntro.
+    iExists _.
+    iDestruct (is_slice_sz with "HtidsS") as "%HtidsSz".
+    rewrite fmap_length in HtidsSz.
+    iFrame "% ∗".
+    iPureIntro.
+    split.
+    { replace (int.nat _) with (S (int.nat idx)); last word.
+      rewrite (take_S_r _ _ tidx); last done.
+      apply Forall_app_2; first done.
+      apply Forall_singleton.
+      apply u64_val_ne in Heqb.
+      unfold not. intros H. rewrite H in Heqb. word.
+    }
+    { destruct (decide (int.Z idx < Z.of_nat (length tids) - 1)); first word.
+      apply Znot_lt_ge in n.
+      assert (Hexists: Exists (λ tidx : u64, tidx = tid) tids).
+      { rewrite Exists_exists. by exists tid. }
+      destruct (Exists_not_Forall (λ tidx : u64, tidx ≠ tid) tids).
+      { apply (Exists_impl _ _ _ Hexists). auto. }
+      replace tids with (take (S (int.nat idx)) tids); last first.
+      { rewrite take_ge; [done | word]. }
+      rewrite (take_S_r _ _ tidx); last done.
+      apply Forall_app_2; first done.
+      apply Forall_singleton.
+      apply u64_val_ne in Heqb.
+      unfold not. intros H. rewrite H in Heqb. word.
+    }
+  }
+  { iExists _.
+    iFrame.
+    iPureIntro.
+    split.
+    { change (int.nat 0) with 0%nat. by rewrite take_0. }
+    split; last done.
+    { apply elem_of_list_lookup in Helem as [i Hlookup].
+      apply lookup_lt_Some in Hlookup. word.
+    }
+  }
+  iIntros "Hloop".
+  iNamed "Hloop".
+  wp_pures.
+  
+  (***********************************************************)
+  (* return idx                                              *)
+  (***********************************************************)
+  wp_load.
+  iApply "HΦ".
+  by iFrame.
+Qed.
 
 (*****************************************************************)
 (* func (txnMgr *TxnMgr) deactivate(sid uint64, tid uint64)      *)
@@ -736,17 +990,174 @@ Proof.
   iNamed "Htxnmgr".
   wp_call.
 
+  (***********************************************************)
+  (* site := txnMgr.sites[sid]                               *)
+  (***********************************************************)
+  wp_loadField.
+  iMod (readonly_load with "HsitesS") as (q) "HsitesS'".
+  iDestruct "Hactive" as "[[HactiveFrag %Hbound] _]".
+  list_elem sitesL (int.nat sid) as site.
+  wp_apply (wp_SliceGet with "[$HsitesS']").
+  { iPureIntro.
+    rewrite list_lookup_fmap.
+    by rewrite Hsite_lookup.
+  }
+  iIntros "[HsitesS' %HsiteVT]".
+  wp_pures.
+
+  (***********************************************************)
+  (* site.latch.Lock()                                       *)
+  (***********************************************************)
+  iDestruct (big_sepL_lookup with "HsitesRP") as "HsiteRP"; first done.
+  iClear (latch) "Hlatch Hlock".
+  iNamed "HsiteRP".
+  wp_loadField.
+  wp_apply (acquire_spec with "[$Hlock]").
+  iIntros "[Hlocked HsiteOwn]".
+  replace (U64 (Z.of_nat _)) with sid by word. 
+  iNamed "HsiteOwn".
+  iDestruct (is_slice_sz with "HactiveL") as "%HactiveSz".
+  rewrite fmap_length in HactiveSz.
+  wp_pures.
+  
   (*****************************************************************)
-  (* sid := getSID(tid)                                            *)
-  (* site := txnMgr.sites[sid]                                     *)
-  (* site.latch.Lock()                                             *)
   (* idx := findTID(tid, site.tidsActive)                          *)
+  (*****************************************************************)
+  wp_loadField.
+  iDestruct (site_active_tids_elem_of with "HactiveAuth HactiveFrag") as "%Hin".
+  rewrite -HactiveLM elem_of_list_to_set in Hin.
+  wp_apply (wp_findTID tid _ tidsactiveL with "[$HactiveL]"); first auto.
+  iIntros (pos) "[HactiveL %Hlookup]".
+  wp_pures.
+  
+  (*****************************************************************)
   (* swapWithEnd(site.tidsActive, idx)                             *)
+  (*****************************************************************)
+  wp_loadField.
+  wp_apply (wp_swapWithEnd with "[HactiveL]"); first by iFrame.
+  iIntros (tids) "[HactiveL %Hperm]".
+  wp_pures.
+  
+  (*****************************************************************)
   (* site.tidsActive = site.tidsActive[:len(site.tidsActive) - 1]  *)
+  (*****************************************************************)
+  wp_loadField.
+  wp_apply (wp_slice_len).
+  wp_pures.
+  wp_loadField.
+  wp_apply (wp_SliceTake).
+  { apply lookup_lt_Some in Hlookup. word. }
+  wp_storeField.
+  wp_loadField.
+
+  (* Open the global invariant to update the local active TIDs. *)
+  iApply fupd_wp.
+  iInv "Hinvgc" as ">HinvgcO" "HinvgcC".
+  iDestruct (big_sepL_lookup_acc with "HinvgcO") as "[HinvgcO HinvgcOAcc]".
+  { by apply sids_all_lookup. }
+  iDestruct "HinvgcO" as (tidsM tidmin') "(HactiveAuth' & HminAuth' & Hmin)".
+  (* Update the set of active tids. *)
+  iDestruct (site_active_tids_agree with "HactiveAuth' HactiveAuth") as %->.
+  iMod (site_active_tids_delete tid with "HactiveFrag HactiveAuth' HactiveAuth") as "[HactiveAuth' HactiveAuth]".
+  (* Close the global invariant. *)
+  iDestruct ("HinvgcOAcc" with "[HactiveAuth' HminAuth' Hmin]") as "HinvgcO".
+  { do 2 iExists _.
+    iFrame "HactiveAuth' HminAuth'".
+    rewrite dom_delete_L.
+    iDestruct (big_sepS_delete with "Hmin") as "[_ H]".
+    { rewrite -HactiveLM.
+      apply elem_of_list_to_set.
+      by eapply elem_of_list_lookup_2.
+    }
+    done.
+  }
+  iMod ("HinvgcC" with "[HinvgcO]") as "_"; first done.
+  iModIntro.
+  
+  (*****************************************************************)
   (* site.latch.Unlock()                                           *)
   (*****************************************************************)
-  
-Admitted.
+  wp_apply (release_spec with "[-HΦ]").
+  { iFrame "Hlock Hlocked".
+    iNext.
+    set idxlast := (word.sub _ _).
+    iExists _, _, _, tids, _.
+    iFrame "Hactive".
+    iFrame.
+    assert (Hidxlast : int.nat idxlast = length tids).
+    { subst idxlast.
+      rewrite (Permutation_length Hperm).
+      rewrite length_delete; last done.
+      assert (H : (int.nat tidsactive.(Slice.sz) > 0)%nat).
+      { rewrite -HactiveSz. apply lookup_lt_Some in Hlookup. lia. }
+      rewrite HactiveSz. word.
+    }
+    iSplitL "HactiveL".
+    { (* Prove [HactiveL]. *)
+      unfold typed_slice.is_slice.
+      unfold list.untype.
+      iDestruct (is_slice_take_cap _ _ _ idxlast with "HactiveL") as "H".
+      { rewrite fmap_length. rewrite last_length. word. }
+      unfold named.
+      iExactEq "H".
+      rewrite -fmap_take.
+      do 2 f_equal.
+      replace (int.nat idxlast) with (length tids).
+      apply take_app.
+    }
+    iSplit.
+    { (* Prove [HactiveLM]. *)
+      iPureIntro.
+      rewrite (list_to_set_perm_L _ (delete (int.nat pos) tidsactiveL)); last done.
+      rewrite dom_delete_L.
+      rewrite -HactiveLM.
+      rewrite delete_take_drop.
+      apply take_drop_middle in Hlookup.
+      rewrite <- Hlookup at 3.
+      do 2 rewrite list_to_set_app_L.
+      rewrite list_to_set_cons.
+      set s1 := (list_to_set (take _ _)).
+      set s2 := (list_to_set (drop _ _)).
+      do 2 rewrite difference_union_distr_l_L.
+      rewrite -Hlookup in HactiveND.
+      apply NoDup_app in HactiveND as [_ [Hnotins1 Hnotins2]].
+      apply NoDup_cons in Hnotins2 as [Hnotins2 _].
+      replace (s1 ∖ {[tid]}) with s1 by set_solver.
+      replace (s2 ∖ {[tid]}) with s2 by set_solver.
+      set_solver.
+    }
+    iPureIntro.
+    split.
+    { (* Prove [HactiveND]. *)
+      apply (NoDup_Permutation_proper _ _ Hperm).
+      rewrite delete_take_drop.
+      apply take_drop_middle in Hlookup.
+      rewrite -Hlookup in HactiveND.
+      apply NoDup_app in HactiveND as [HND1 [Hnotin1 HND2]].
+      apply NoDup_cons in HND2 as [_ HND2].
+      apply NoDup_app.
+      split; first done.
+      split; last done.
+      set_solver.
+    }
+    split.
+    { (* Prove [HtidOrder] *)
+      apply Forall_cons_2; first by apply Forall_inv in HtidOrder.
+      apply Forall_inv_tail in HtidOrder.
+      apply (Forall_Permutation _ _ _ Hperm).
+      by apply Forall_delete.
+    }
+    split; last done.
+    { (* Prove [HtidFree]. *)
+      simpl.
+      intros tidx Htidx.
+      apply not_elem_of_weaken with (dom (gset u64) tidsactiveM); last set_solver.
+      auto.
+    }
+  }
+  wp_pures.
+  by iApply "HΦ".
+Qed.
   
 (*****************************************************************)
 (* func (txnMgr *TxnMgr) getMinActiveTIDSite(sid uint64) uint64  *)
@@ -913,6 +1324,7 @@ Proof.
   rewrite -HtidsactiveSz in Helem HtidminLe.
   rewrite firstn_all in Helem HtidminLe.
 
+  (* Prove that we can safely update the local lower bound. *)
   assert (Hle : int.Z tidmin ≤ int.Z tidmin').
   { apply elem_of_cons in Helem.
     destruct Helem.
@@ -1041,6 +1453,7 @@ Proof.
       { iApply (big_sepL_impl with "Htidlbs").
         iModIntro.
         iIntros (iN sid) "Hlookup Htidlb".
+        (* Weaken all previous lower bounds. *)
         iApply (site_min_tid_lb_weaken with "Htidlb").
         word.
       }
@@ -1057,6 +1470,7 @@ Proof.
       iSplitL "Htidlbs"; first done.
       simpl.
       iSplit; last done.
+      (* Weaken the current lower bound. *)
       iApply (site_min_tid_lb_weaken with "Htidlb").
       word.
   }
